pulse/share/steel/examples/pulse/bug-reports/PulseLambdas.fst
@@ -1,0 +1,60 @@
+module PulseLambdas
+open Pulse.Lib.Pervasives
+
+// [@@expect_failure]
+// ```pulse
+// fn test_tot_function (x:int)
+// : int
+// = { //should allow nullary "lambdas"
+//     x + 1
+//   }
+// ```
+
+// ```pulse
+// fn swap (#a:Type0) (x y:ref a) (#vx #vy:erased a)
+//     requires pts_to x vx ** pts_to y vy
+//     ensures pts_to x vy ** pts_to y vx
+// {
+//   let vx = !x;
+//   let vy = !y;
+//   x := vy;
+//   y := vx;
+// } 
+// ```
+
+let swap_fun a = x:ref a -> y:ref a -> #vx:erased a -> #vy:erased a -> stt unit
+    (requires pts_to x vx ** pts_to y vy)
+    (ensures fun _ -> pts_to x vy ** pts_to y vx)
+
+
+```pulse
+fn test_top_level_lambda (#a:Type0)
+  : swap_fun a
+  = (x y:_) (#vx #vy:_)
+    {
+      let vx = !x;
+      let vy = !y;
+      x := vy;
+      y := vx;
+    }
+```
+
+// [@@expect_failure]
+// ```pulse
+// fn test_inner_lambda (#a:Type0)
+//                      (x y:ref int)
+// requires pts_to x 'vx ** pts_to y 'vy
+// ensures  pts_to x 'vy ** pts_to y 'vx
+// {
+//   fn write_helper (#a:Type) (x:ref a) (n:a)
+//     requires pts_to x 'vx
+//     ensures  pts_to x n
+//   {
+//     x := n;
+//   };
+//   let vx = !x;
+//   let vy = !y;
+//   write_helper x vy;
+//   write_helper y vy;
+// } 
+// ```
